cambios

Auxiliary/Map.dfy
@@ -6,11 +6,17 @@ It encapsulates the Dafny map
 Contains ghost functions to assist in the verification of the properties of the map and on the computational cost of its operations
 Has the typical `map` operations
 */
-type Map< T1(==), T2(==) > {
+type Map< T0(==), T1(==) > {
 
-  ghost function Model():map<T1,T2>
+  ghost function Model():map<T0,T1>
 
-  ghost function Universe():map<T1,T2>
+  ghost function Universe():map<T0,T1>
+
+  ghost function Keys():set<T0>
+  { Model().Keys }
+
+  ghost function Values():set<T1>
+  { Model().Values }
 
   ghost function Valid():bool
   {
@@ -19,7 +25,7 @@ type Map< T1(==), T2(==) > {
     (Cardinality() <= |Universe()|)
   }
 
-  ghost function UBSize0():nat
+  ghost function UBSize():nat
   { Cardinality() }
 
   ghost function Cardinality():(c:nat)
@@ -27,42 +33,115 @@ type Map< T1(==), T2(==) > {
   { |Model()| }
 
 
-  method {:axiom} Get(key:T1, ghost counter_in:nat) returns (val:T2, ghost counter_out:nat)
+  method {:axiom} Get(key:T0, ghost counter_in:nat) returns (val:T1, ghost counter_out:nat)
     requires Valid()
     ensures key in Model().Keys
     ensures val == Model()[key]
-    ensures counter_out == counter_in + UBSize0()
+    ensures counter_out == counter_in + UBSize()
 
-  method {:axiom} Insert(key:T1, val:T2, ghost counter_in:nat) returns (r:Map<T1,T2>, ghost counter_out:nat)
+  method {:axiom} Insert(key:T0, val:T1, ghost counter_in:nat) returns (r:Map<T0,T1>, ghost counter_out:nat)
     requires Valid()
     ensures r.Model() == Model()[key := val]
     ensures r.Universe() == Universe()[key := val]
-    ensures counter_out == counter_in + UBSize0()
+    ensures counter_out == counter_in + UBSize()
 
-  method {:axiom} Remove(key:T1, ghost counter_in:nat) returns (r:Map<T1,T2>, ghost counter_out:nat)
+  method {:axiom} Remove(key:T0, ghost counter_in:nat) returns (r:Map<T0,T1>, ghost counter_out:nat)
     requires Valid()
     ensures r.Model() == Model() - {key}
-    ensures counter_out == counter_in + UBSize0()
+    ensures counter_out == counter_in + UBSize()
 
-  method {:axiom} nPairs(ghost counter_in:nat) returns (size:int, ghost counter_out:nat)
+  method {:axiom} nPairs(ghost counter_in:nat) returns (n:int, ghost counter_out:nat)
     requires Valid()
-    ensures size == |Model()|
+    ensures n == |Model()|
     ensures counter_out == counter_in + 1
 
-  method {:axiom} ContainsKey(key:T1, ghost counter_in:nat) returns (b:bool, ghost counter_out:nat)
+  method {:axiom} ContainsKey(key:T0, ghost counter_in:nat) returns (b:bool, ghost counter_out:nat)
     requires Valid()
     ensures b == (key in Model())
-    ensures counter_out == counter_in + UBSize0()
+    ensures counter_out == counter_in + UBSize()
 
   method {:axiom} Empty(ghost counter_in:nat) returns (b:bool, ghost counter_out:nat)
     requires Valid()
     ensures b == (|Model()| == 0)
     ensures counter_out == counter_in + 1
 
-  method {:axiom} Copy(ghost counter_in:nat) returns (r:Map<T1,T2>, ghost counter_out:nat)
+  method {:axiom} Copy(ghost counter_in:nat) returns (r:Map<T0,T1>, ghost counter_out:nat)
     requires Valid()
     ensures r.Model() == Model()
     ensures r.Universe() == Model()
-    ensures counter_out == counter_in + UBSize0()
+    ensures counter_out == counter_in + UBSize()
+
+}
+
+
+// Maps whose keys are maps
+type Map_Map_T< T0(==), T1(==), T2(==) > {
+
+  ghost function Model():map<map<T0, T1>,T2>
+
+  ghost function Universe():map<map<T0, T1>,T2>
+
+  ghost function Keys():set<map<T0, T1>>
+  { Model().Keys }
+
+  ghost function Values():set<T2>
+  { Model().Values }
+
+  ghost function Valid():bool
+  {
+    (Model().Keys <= Universe().Keys) &&
+    (forall k | k in Model().Keys :: Model()[k] == Universe()[k]) &&
+    (Cardinality() <= |Universe()|)
+  }
+
+  ghost function UBSize():nat
+  { Cardinality() * UBSize_Keys() }
+
+  ghost function {:axiom} UBSize_Keys():nat
+    ensures forall k | k in Universe().Keys :: UBSize_Keys() >= |k|
+    ensures exists k :: k in Universe().Keys && UBSize_Keys() == |k|
+
+  ghost function Cardinality():(c:nat)
+  ensures 0 <= c
+  { |Model()| }
+
+
+  method {:axiom} Get(key:map<T0, T1>, ghost counter_in:nat) returns (val:T2, ghost counter_out:nat)
+    requires Valid()
+    ensures key in Model().Keys
+    ensures val == Model()[key]
+    ensures counter_out == counter_in + UBSize()
+
+  method {:axiom} Insert(key:map<T0, T1>, val:T2, ghost counter_in:nat) returns (r:Map_Map_T<T0,T1,T2>, ghost counter_out:nat)
+    requires Valid()
+    ensures r.Model() == Model()[key := val]
+    ensures r.Universe() == Universe()[key := val]
+    ensures counter_out == counter_in + UBSize()
+
+  method {:axiom} Remove(key:map<T0, T1>, ghost counter_in:nat) returns (r:Map_Map_T<T0,T1,T2>, ghost counter_out:nat)
+    requires Valid()
+    ensures r.Model() == Model() - {key}
+    ensures counter_out == counter_in + UBSize()
+
+  method {:axiom} nPairs(ghost counter_in:nat) returns (n:int, ghost counter_out:nat)
+    requires Valid()
+    ensures n == |Model()|
+    ensures counter_out == counter_in + 1
+
+  method {:axiom} ContainsKey(key:map<T0, T1>, ghost counter_in:nat) returns (b:bool, ghost counter_out:nat)
+    requires Valid()
+    ensures b == (key in Model())
+    ensures counter_out == counter_in + UBSize()
+
+  method {:axiom} Empty(ghost counter_in:nat) returns (b:bool, ghost counter_out:nat)
+    requires Valid()
+    ensures b == (|Model()| == 0)
+    ensures counter_out == counter_in + 1
+
+  method {:axiom} Copy(ghost counter_in:nat) returns (r:Map_Map_T<T0,T1,T2>, ghost counter_out:nat)
+    requires Valid()
+    ensures r.Model() == Model()
+    ensures r.Universe() == Model()
+    ensures counter_out == counter_in + UBSize()
 
 }
