Reduction/PolynomialSetCoverToCDPC.dfy
@@ -5,8 +5,8 @@ include "../Auxiliary/Set.dfy"
 include "../Auxiliary/Map.dfy"
 include "../Reduction/ReductionSetCoverToCDPC.dfy"
 
-method SetCoverToCDPC_Method(U:set<int>, S:set<set<int>>, k:nat) returns (r:(map<Candidate, bool>, map<Candidate, int>, set<int>, real, real, real, real))
-  requires forall s | s in S :: s <= U
-  requires isCover(U, S)
-  ensures r == SetCoverToCDPC(U, S, k)
+method SetCoverToCDPC_Method(U:Set<int>, S:SetSet<int>, k:nat) returns (r:(Map_Map_T<int, bool, bool>, Map_Map_T<int, bool, int>, Set<int>, real, real, real, real), ghost counter:nat)
+  requires forall s | s in S.Model() :: s <= U.Model()
+  requires isCover(U.Model(), S.Model())
+  ensures (r.0.Model(), r.1.Model(), r.2.Model(), r.3, r.4, r.5, r.6) == SetCoverToCDPC(U.Model(), S.Model(), k)
 
