Verification/VerificationCDPC.dfy
@@ -5,12 +5,18 @@ include "../Auxiliary/Set.dfy"
 include "../Auxiliary/Map.dfy"
 
 
-method verifyCDPC(f:map<Candidate, bool>, g:map<Candidate, int>, P:set<int>, a:real, b:real, x:real, y:real, interview:Interview) returns (r:bool)
-  requires f.Keys == g.Keys
-  requires forall c:Candidate | c in f.Keys :: (P <= c.Keys)
+method verifyCDPC(f:Map_Map_T<int, bool, bool>, g:Map_Map_T<int, bool, int>, P:Set<int>, a:real, b:real, x:real, y:real, interview:Interview) returns (r:bool, ghost counter:nat)
+  requires f.Keys() == g.Keys()
+  requires forall c:Candidate | c in f.Keys() :: (P.Model() <= c.Keys)
   requires 0.0 <= a <= b <= 1.0
   requires 0.0 <= x <= y <= 1.0
-  ensures r == certificateCDPC(f, g, P, a, b, x, y, interview)
+  ensures r == certificateCDPC(f.Model(), g.Model(), P.Model(), a, b, x, y, interview)
   {
+    if (interview == Empty) {
+      
+    }
+    else {
+      
+    }
     assume false;
   }
